upd

coqimp/ext/rellogic_soundness.v
@@ -20,6 +20,16 @@ Require Import refinement.
 Require Import rellogic.
 Require Import lemmas_comp.
 
+(** Auxiliary Lemmas *)
+Lemma last_Kq_cons_Q_same :
+  forall A (Kq : list A) Q Q',
+    last Kq Q = last (Q :: Kq) Q'.
+Proof.
+  induction Kq; intros; simpl; eauto.
+  destruct Kq; eauto.
+Qed.
+
+(** Well formed Instruction Seqence Soundness *)
 Definition get_index_fcall (rls : RelState) :=
   match rls with
   | (LS, HS, A, w) => w
@@ -53,6 +63,7 @@ Lemma wf_insSeq_rel_soundness :
 Proof.
 Admitted.
 
+(** Well formed CodeHeap Soundness *)
 Lemma wf_cdhp_rel_sound : forall Spec C,
     rel_wf_cdhp Spec C -> cdhp_rel_sound Spec C.
 Proof.
@@ -64,10 +75,180 @@ Proof.
   eapply wf_insSeq_rel_soundness; eauto.
 Qed.
 
-Lemma function_correctness :
+(** Functional Safety *)
+Fixpoint WFST (Q : relasrt) (Kq : list relasrt) (Spec : Funspec) (C : XCodeHeap) :=
+  match Kq with
+  | nil => (Q ⇒ RAprim Pdone ⋆ RAtrue)
+  | Q' :: Kq' => forall S HS A w, (S, HS, A, w) ||= Q ->
+                              exists f I, (getregs S) r15 = Some (W f) /\ LookupXC C (f +ᵢ ($ 8)) I /\ 
+                                   rel_safety_insSeq Spec (w, (1 + get_insSeqLen I)%nat)
+                                                     (C, S, f +ᵢ ($ 8), f +ᵢ ($ 12)) (A, HS) Q' /\
+                                   WFST Q' Kq' Spec C
+  end.
+
+CoInductive rel_safety_WFST : Index -> (XCodeHeap * State * Word * Word) -> (primcom * HState) ->
+                              relasrt -> list relasrt -> Funspec -> Prop :=
+| cons_safety : forall idx C S pc npc A HS Q Kq Spec,  
+    legal_com (C pc) -> legal_com (C npc) -> WFST Q Kq Spec C -> 
+    (* not call ret *)
+    (
+      forall f aexp rd i,
+        (C pc = Some (c (cntrans i)) \/ C pc = Some (c (cjumpl aexp rd)) \/ C pc = Some (c (cbe f))) ->
+        (
+          (* progress *)
+          exists S' pc' npc',
+            LP__ (C, (S, pc, npc)) tau (C, (S', pc', npc'))
+        ) /\
+        (
+          (* preservation *)
+          forall S' pc' npc',
+            LP__ (C, (S, pc, npc)) tau (C, (S', pc', npc')) ->
+            (
+              (
+                exists idx1, (idx1 ⩹ idx) /\ rel_safety_WFST idx1 (C, S', pc', npc') (A, HS) Q Kq Spec
+              )
+              \/
+              (
+                exists HS' idx1, exec_prim (A, HS) (Pdone, HS')
+                            /\ rel_safety_WFST idx1 (C, S', pc', npc') (Pdone, HS') Q Kq Spec
+              )
+            )
+        )
+    ) ->
+    (* call *)
+    (
+      forall f,
+        C pc = Some (c (ccall f)) ->
+        (
+          (* progress *)
+          exists S1 S2 pc1 pc2 npc1 npc2,
+            LP__ (C, (S, pc, npc)) tau (C, (S1, pc1, npc1)) /\
+            LP__ (C, (S1, pc1, npc1)) tau (C, (S2, pc2, npc2))
+        ) /\
+        (
+          (* preservation *)
+          forall S1 S2 pc1 pc2 npc1 npc2,
+            LP__ (C, (S, pc, npc)) tau (C, (S1, pc1, npc1)) ->
+            LP__ (C, (S1, pc1, npc1)) tau (C, (S2, pc2, npc2)) ->
+            exists idx1 idx2 A' HS' Q0,
+              ((idx1 ⩹ idx2 /\ idx2 ⩹ idx /\  A' = A /\ HS = HS') \/ (exec_prim (A, HS) (A', HS'))) /\
+              rel_safety_WFST idx1 (C, S2, pc2, npc2) (A', HS') Q0 (Q :: Kq) Spec
+        )
+    ) ->
+    (* retl *)
+    (
+      C pc = Some (c cretl) ->
+      (
+          (* progress *)
+          exists S1 S2 pc1 pc2 npc1 npc2,
+            LP__ (C, (S, pc, npc)) tau (C, (S1, pc1, npc1)) /\
+            LP__ (C, (S1, pc1, npc1)) tau (C, (S2, pc2, npc2))
+      ) /\
+      (
+          (* preservation *)
+          forall S1 S2 pc1 pc2 npc1 npc2,
+            LP__ (C, (S, pc, npc)) tau (C, (S1, pc1, npc1)) ->
+            LP__ (C, (S1, pc1, npc1)) tau (C, (S2, pc2, npc2)) ->
+            exists idx1 idx2 A' HS' w ,
+              ((idx1 ⩹ idx2 /\ idx2 ⩹ idx /\ A' = A /\ HS = HS') \/ (exec_prim (A, HS) (A', HS'))) /\
+              (S2, HS', A', w) ||= Q /\ 
+              (
+                (Kq = nil /\ A' = Pdone /\ (0%nat, 0%nat) ⩹ idx1 /\
+                 (exists f', getregs S2 r15 = Some (W f') /\ pc2 = f' +ᵢ ($ 8) /\ npc2 = f' +ᵢ ($ 12))) \/
+                (exists Q' Kq', Kq = Q' :: Kq' /\ rel_safety_WFST idx1 (C, S2, pc2, npc2) (A', HS') Q' Kq' Spec)
+              )
+      )
+    ) ->
+    rel_safety_WFST idx (C, S, pc, npc) (A, HS) Q Kq Spec.
+
+Lemma function_correctness_aux' :
+    forall P Q Spec S HS A w pc I C Kq,
+      rel_safety_insSeq Spec (w, (1 + get_insSeqLen I)%nat) (C, S, pc, pc +ᵢ ($ 4)) (A, HS) Q -> 
+      LookupXC C pc I ->
+      (S, HS, A, w) ||= P -> WFST Q Kq Spec C ->
+      rel_safety_WFST (w, (1 + get_insSeqLen I)%nat) (C, S, pc, pc +ᵢ ($ 4)) (A, HS) Q Kq Spec.
+Proof.
+Admitted.
+
+Lemma function_correctness_aux :
+  forall P Q Spec S HS A w pc I C Kq,
+    insSeq_rel_sound Spec P pc I Q -> LookupXC C pc I ->
+    cdhp_rel_sound Spec C -> (S, HS, A, w) ||= P -> WFST Q Kq Spec C ->
+    rel_safety_WFST (w, (1 + get_insSeqLen I)%nat) (C, S, pc, pc +ᵢ ($ 4)) (A, HS) Q Kq Spec.
+Proof.
+  intros.
+  unfolds insSeq_rel_sound.
+  lets Hrel_safety_insSeq : H0.
+  eapply H in Hrel_safety_insSeq; clear H; eauto.
+  eapply function_correctness_aux'; eauto.
+Qed. 
+
+Lemma rel_safety_WFST_impl_rel_safety :
+  forall idx C S pc npc A HS Q Kq Spec Q',
+    rel_safety_WFST idx (C, S, pc, npc) (A, HS) Q Kq Spec ->
+    Q' = last Kq Q ->
+    rel_safety (length Kq) idx (C, S, pc, npc) (A, HS) Q'.
+Proof.
+  cofix Hp; intros.
+  inv H.
+  econstructor; intros; eauto.
+  {
+    (* C pc = i \/ jmpl aexp rd \/ be f *)
+    clear H15 H16.
+    eapply H14 in H.
+    simpljoin1.
+    split; eauto.
+
+    intros.
+    eapply H0 in H1; eauto.
+    destruct H1.
+    {
+      simpljoin1; left.
+      exists x2.
+      split; eauto.
+    }
+    {
+      simpljoin1.
+      right.
+      exists x2 x3.
+      eauto.
+    }
+  }
+  {
+    (* C pc = call f *)
+    clear H14 H16.
+    eapply H15 in H.
+    simpljoin1.
+    split.
+    do 6 eexists.
+    split; eauto.
+
+    intros.
+    eapply H0 with (S1 := S1) in H2; eauto.
+    simpljoin1.
+    destruct H2.
+    do 4 eexists.
+    split; eauto.
+    assert ((Nat.succ (length Kq) = length (Q :: Kq))%nat); eauto.
+    rewrite H5.
+    eapply Hp; eauto.
+    eapply last_Kq_cons_Q_same; eauto.
+
+    do 4 eexists.
+    split; eauto.
+    assert ((Nat.succ (length Kq) = length (Q :: Kq))%nat); eauto.
+    rewrite H5.
+    eapply Hp; eauto.
+    eapply last_Kq_cons_Q_same; eauto.
+  }
+  {
+    (* C pc = retl *)
+  }
+   
+Theorem function_correctness :
   forall P Q Spec S HS A w pc I C,
     insSeq_rel_sound Spec P pc I Q -> LookupXC C pc I ->
-    cdhp_rel_sound Spec C -> (S, HS, A, w) ||= P ->
+    cdhp_rel_sound Spec C -> (S, HS, A, w) ||= P -> Q ⇒ RAprim Pdone ⋆ RAtrue ->
     rel_safety 0%nat (w, (1 + get_insSeqLen I)%nat) (C, S, pc, pc +ᵢ ($ 4)) (A, HS) Q.
 Proof.
 Admitted.
